Reorganisation: the generated induction principles are now in place.

theories/datatypes_properties.v
@@ -146,15 +146,21 @@ Definition eqvalueP : Equality.axiom value_eqb :=
 Canonical Structure value_eqMixin := EqMixin eqvalueP.
 Canonical Structure value_eqType := Eval hnf in EqType value value_eqMixin.
 
-(* TODO: [basic_instruction_rect'] *)
+(** Induction scheme for [basic_instruction]. **)
+Definition basic_instruction_rect' :=
+  ltac:(rect'_build basic_instruction_rect).
 
-(* TODO:
-Scheme Equality for basic_instruction.
-Definition eqglobal_typeP := eq_dec_Equality_axiom global_type_eq_dec.
-*)
-Parameter basic_instruction_eqb : basic_instruction -> basic_instruction -> bool.
+Definition basic_instruction_ind' (P : basic_instruction -> Prop) :=
+  @basic_instruction_rect' P.
 
-Parameter eqbasic_instructionP : Equality.axiom basic_instruction_eqb.
+Definition basic_instruction_eq_dec : forall e1 e2 : basic_instruction,
+  {e1 = e2} + {e1 <> e2}.
+Proof. decidable_equality_using basic_instruction_rect'. Defined.
+
+Definition basic_instruction_eqb cl1 cl2 : bool :=
+  basic_instruction_eq_dec cl1 cl2.
+Definition eqbasic_instructionP : Equality.axiom basic_instruction_eqb :=
+  eq_dec_Equality_axiom basic_instruction_eq_dec.
 
 Canonical Structure basic_instruction_eqMixin := EqMixin eqbasic_instructionP.
 Canonical Structure basic_instruction_eqType :=
@@ -204,149 +210,6 @@ Canonical Structure store_record_eqMixin := EqMixin eqstore_recordP.
 Canonical Structure store_record_eqType := Eval hnf in EqType store_record store_record_eqMixin.
 
 (** Induction scheme for [administrative_instruction]. **)
-Section administrative_instruction_rect'.
-
-Definition curry A B C (f : A -> B -> C) (ab : A * B) :=
-  let: (a, b) := ab in
-  f a b.
-
-Definition uncurry A B C (f : A * B -> C) a b := f (a, b).
-
-Lemma curry_uncurry : forall A B C (f : A * B -> C) ab,
-  curry (uncurry f) ab = f ab.
-Proof. by move=> A B C f [a b]. Qed.
-
-Lemma uncurry_curry : forall A B C (f : A -> B -> C) a b,
-  uncurry (curry f) a b = f a b.
-Proof. by []. Qed.
-
-(** Given an induction principle, return the number of cases of the type. **)
-Ltac count_cases rect :=
-  let rec count_args rectf :=
-    lazymatch rectf with
-    | forall a, False => constr:(0)
-    | _ -> ?rectf' =>
-      let r := count_args rectf' in
-      constr:(r.+1)
-    end in
-  lazymatch type of rect with
-  | forall P : ?t -> Type, @?rectf P =>
-    let r := constr:(rectf (fun _ : t => False)) in
-    let r := eval simpl in r in
-    count_args r
-  end.
-
-Ltac rect'_type rect :=
-  let added_hyp t ta :=
-    lazymatch ta with
-    | list t => constr:(@TProp.Forall t)
-    | option t => constr:(fun P (o : ta) => forall a : t, o = Some a -> P a)
-    | _ => constr:(fun (_ : t -> Type) (_ : ta) => True)
-    end in
-  let add_hyp t ta P a r :=
-    let h := added_hyp t ta in
-    let h := constr:(h P a) in
-    let h := eval simpl in h in
-    lazymatch h with
-    | True => r
-    | _ => constr:(h -> r)
-    end in
-  let set_hyp t ta P a r :=
-    let r := add_hyp t ta P a r in
-    exact r in
-  let update_hyp t hyp :=
-    lazymatch hyp with
-    | fun P => P _ => constr:(hyp)
-    | fun P => forall a1 : ?t1, P (?C a1) =>
-      constr:(fun P : t -> Type => forall a1 : t1,
-        ltac:(set_hyp t t1 P a1 (P (C a1))))
-    | fun P => forall (a1 : ?t1) (a2 : ?t2), P (?C a1 a2) =>
-      constr:(fun P : t -> Type => forall (a1 : t1) (a2 : t2),
-        ltac:(set_hyp t t1 P a1
-          ltac:(add_hyp t t2 P a2 (P (C a1 a2)))))
-    | fun P => forall (a1 : ?t1) (a2 : ?t2) (a3 : ?t3), P (?C a1 a2 a3) =>
-      constr:(fun P : t -> Type => forall (a1 : t1) (a2 : t2) (a3 : t3),
-        ltac:(set_hyp t t1 P a1
-          ltac:(add_hyp t t2 P a2
-            ltac:(add_hyp t t3 P a3 (P (C a1 a2 a3))))))
-    | fun P => forall (a1 : ?t1) (a2 : ?t2) (a3 : ?t3) (a4 : ?t4), P (?C a1 a2 a3 a4) =>
-      constr:(fun P : t -> Type => forall (a1 : t1) (a2 : t2) (a3 : t3) (a4 : t4),
-        ltac:(set_hyp t t1 P a1
-          ltac:(add_hyp t t2 P a2
-            ltac:(add_hyp t t3 P a3
-              ltac:(add_hyp t t4 P a4 (P (C a1 a2 a3 a4)))))))
-    | fun P => forall (a1 : ?t1) (a2 : ?t2) (a3 : ?t3) (a4 : ?t4) (a5 : ?t5), P (?C a1 a2 a3 a4 a5) =>
-      constr:(fun P : t -> Type => forall (a1 : t1) (a2 : t2) (a3 : t3) (a4 : t4) (a5 : t5),
-        ltac:(set_hyp t t1 P a1
-          ltac:(add_hyp t t2 P a2
-            ltac:(add_hyp t t3 P a3
-              ltac:(add_hyp t t4 P a4
-                ltac:(add_hyp t t4 P a4 (P (C a1 a2 a3 a4 a5))))))))
-    | fun P => forall (a1 : ?t1) (a2 : ?t2) (a3 : ?t3) (a4 : ?t4) (a5 : ?t5) (a6 : ?t6), P (?C a1 a2 a3 a4 a5 a6) =>
-      constr:(fun P : t -> Type => forall (a1 : t1) (a2 : t2) (a3 : t3) (a4 : t4) (a5 : t5) (a6 : t6),
-        ltac:(set_hyp t t1 P a1
-          ltac:(add_hyp t t2 P a2
-            ltac:(add_hyp t t3 P a3
-              ltac:(add_hyp t t4 P a4
-                ltac:(add_hyp t t5 P a5
-                  ltac:(add_hyp t t6 P a6 (P (C a1 a2 a3 a4 a5 a6)))))))))
-    end in
-  let rec map_hyps t rectf :=
-    lazymatch rectf with
-    | fun P => forall a : t, P a => constr:(rectf)
-    | fun P => @?hyp P -> @?rectf' P =>
-      let r := update_hyp t hyp in
-      let r' := map_hyps t rectf' in
-      constr:(fun P => r P -> r' P)
-    end in
-  lazymatch type of rect with
-  | forall P : ?t -> Type, @?rectf P =>
-    let r := map_hyps t rectf in
-    let r := constr:(forall P, r P) in
-    eval simpl in r
-  end.
-
-Ltac rect'_build rect :=
-  let t :=
-    lazymatch type of rect with
-    | forall P : ?t -> Type, _ => t
-    end in
-  let g := rect'_type rect in
-  refine (_ : g);
-  let P := fresh "P" in
-  intro P;
-  repeat lazymatch goal with
-  | |- forall a : t, P a => idtac
-  | |- _ -> _ => intro
-  end;
-  let rect := fresh "rect" in
-  fix rect 1;
-  let rect_list := fresh "rect_list" in
-  refine (
-    let rect_list :=
-      fix rect_list es : TProp.Forall P es :=
-        match es with
-        | [::] => TProp.Forall_nil _
-        | e :: l => TProp.Forall_cons (rect e) (rect_list l)
-        end in _);
-  let do_it := clear rect rect_list; auto in
-  let use_hyps :=
-    intros;
-    repeat match goal with
-    | a : t |- _ =>
-      lazymatch goal with
-      | H : P a |- _ => fail
-      | _ => move: (rect a) => ?
-      end
-    | l : list t |- _ =>
-      lazymatch goal with
-      | H : TProp.Forall P l |- _ => fail
-      | _ => move: (rect_list l) => ?
-      end
-    | o : option t |- _ => destruct o
-    end in
-  case; try solve [ do_it | use_hyps; do_it ].
-  
 Definition administrative_instruction_rect' :=
   ltac:(rect'_build administrative_instruction_rect).
 
@@ -357,7 +220,8 @@ Definition administrative_instruction_eq_dec : forall e1 e2 : administrative_ins
   {e1 = e2} + {e1 <> e2}.
 Proof. decidable_equality_using administrative_instruction_rect'. Defined.
 
-Definition administrative_instruction_eqb cl1 cl2 : bool := administrative_instruction_eq_dec cl1 cl2.
+Definition administrative_instruction_eqb cl1 cl2 : bool :=
+  administrative_instruction_eq_dec cl1 cl2.
 Definition eqadministrative_instructionP : Equality.axiom administrative_instruction_eqb :=
   eq_dec_Equality_axiom administrative_instruction_eq_dec.
 
